\documentclass[11pt, oneside]{article} 
\usepackage{geometry}
\geometry{letterpaper} 
\usepackage{graphicx}
	
\usepackage{amssymb}
\usepackage{amsmath}
\usepackage{parskip}
\usepackage{color}
\usepackage{hyperref}

\graphicspath{{/Users/telliott/Github/figures/}}

\title{Quotients}
\date{}

\begin{document}
\maketitle
\Large


%[my-super-duper-separator]

\subsection*{Boas}

If $g$ is analytic, not equal to $0$ at $z_0$, and $h(z_0) = 0$, then
\[ R(z_0) = \frac{g(z_0)}{h'(z_0)} \]

\subsection*{example}

\label{sec:ex31R}

Find $R(i)$ for 
\[ f(z) = \frac{\sin z}{1 - z^4} \]
Using the rule:
\[ g(i) = \sin i = \frac{1}{2} (e^{i \cdot i} - e^{-i \cdot i}) \]
\[ = \frac{1}{2} (e^{-1} - e^{1}) = -i \sinh 1 \]

\[ h'(z) = 4z^3 \bigg |_i = 4(- i) \]
Dividing 
\[ R(i) = \frac{1}{4} \sinh 1 \]

\subsection*{Kaplan}

If $A(z)$ and $B(z)$ are analytic in a neighborhood of $z_0$, $A(z_0) \ne 0$, and $B(z)$ has a zero at $z_0$ of order 1, then
\[ f(z) = \frac{A(z)}{B(z)} \]
has a pole of first order at $z_0$ and
\[ \text{Res } [f(z),z_0] = \frac{A(z_0)}{B'(z_0)} \]

\subsection*{example}

\label{sec:ex10R}

\[ f(z) = \frac{1}{z^2 + 1} = \frac{1}{(z - i)(z + i)} \]
\[ B = z^2 + 1, \ \ \ B' = 2z \]
\[ \text{Res } [f(z),z=i] = \frac{1}{2i} \]
\[ \text{Res } [f(z),z=-i] = -\frac{1}{2i} \]

\subsection*{example}

\label{sec:ex27R}

\[ f(z) = \frac{z e^z}{z^2 - 1} \]
Both top and bottom are analytic.  The poles of $B(z)$ are at $\pm \ 1$.  $A(z) \ne 0$ at those points.  We have 
\[ \frac{A(z)}{B'(z)} = \frac{z e^z}{2z} \]
\[ \frac{z e^z}{2z} \ \bigg |_{z=1} = \frac{e}{2} \]
\[ \frac{z e^z}{2z} \ \bigg |_{z=-1} = e^{-1} \]

\textbf{RULE IV}  If $A(z)$ and $B(z)$ are analytic in a neighborhood of $z_0$, $A(z_0) \ne 0$, and $B(z)$ has a zero at $z_0$ of order 2, then
\[ \text{Res } [f(z),z_0] = \frac{6A' B'' - 2AB'''}{3B''^2} \]

\subsection*{example}

\label{sec:ex30R}

\[ f(z) = \frac{e^z}{z(z-1)^2} \]
\[ B = z(z^2 - 2z + 1) = z^3 - 2z^2 + z \]
\[ B' = 3z^2 - 4z + 1 \]
\[ B'' = 6z - 4 \]
\[ B''' = 6 \]

So
\[ \frac{6A' B'' - 2AB'''}{3B''^2} = \frac{6(e^z)(6z-4) - 2e^z(6)}{3(6z-4)^2} \ \]
Evaluate at $z=1$:
\[ \frac{6e(2) - 2e(6)}{12} = 0 \]
So only the pole at $z=0$ contributes.


\end{document}